lean/Splay.lean
@@ -1,4 +1,8 @@
+import Std.Data.AssocList
+
+import Splay.STree
 import Splay.SplayBST
+import Splay.Assoc
 ---- TODO section the bst invariant, proving insert_BST ----
 
 theorem splay_BST (t : STree α) (key : Nat)
@@ -17,6 +21,23 @@ theorem insert_BST (t : STree α) (key : Nat) (val : α)
   assumption
 
 ------- TODO section doc; model verification -------
+
+---- association lists
+theorem elements_splay {α : Type} (t : STree α) (k : Nat) (hbst : BST t)
+  : t.elements = (t.splay k).elements := by
+  apply elements_splay_impl t k hbst
+
+theorem bound_relate {α : Type} (t : STree α) (k : Nat) (hbst : BST t)
+  : t.bound k = bound_assoc t.abs k := by
+  apply bound_relate_impl t k hbst
+
+theorem lookup_relate {α : Type} (t : STree α) (k : Nat) (hbst : BST t)
+  : (t.lookup? k).1 = lookup_assoc t.abs k := by
+  apply lookup_relate_impl t k hbst
+
+theorem insert_relate {α : Type} (t : STree α) (k : Nat) (v : α) (hbst : BST t)
+  : (t.insert k v).abs = insert_assoc t.abs k v := by
+  apply insert_relate_impl t k v hbst
 
 ------- TODO section doc; algebraic spec -------
 
